f2effect: cleanups and reformatting
Ignore-this: e66c872629a22ff4156f22d42d1726a7

darcs-hash:20131015064438-08f32-b15fb874e83efa2dd895065df8aa4cbf5b097cd1

done/Iron/Language/SystemF2Effect/Type/Exp/Base.v
@@ -6,7 +6,7 @@ Require Export Iron.Language.SystemF2Effect.Type.Exp.TyCap.
 
 (********************************************************************)
 (* Type Expressions. *)
-Inductive ty  : Type :=
+Inductive ty  : Type  := 
  | TVar      : nat    -> ty
  | TForall   : ki     -> ty -> ty
  | TApp      : ty     -> ty -> ty
@@ -49,58 +49,68 @@ Notation TRef R T    := (TCon2 TyConRef R T).
 (* Predicates to test whether types have specific forms. *)
 
 (* Check whether a type is a variable with the given index. *)
-Definition isTVar (n : nat) (t : ty) : bool
- := match t with
-    | TVar n'               => beq_nat n n'
-    | _                     => false
-    end.
+Definition isTVar_b   (n : nat) (t : ty) :=
+ match t with
+ | TVar n' => beq_nat n n'
+ | _       => false
+ end.
+
+
+Definition isTVar  (n : nat) (t : ty)
+ := isTVar_b n t = true.
 
 
 (* If we know a type is a variable, then it is one.. *)
 Lemma isTVar_form
  :  forall i t
- ,  true = isTVar i t
+ ,  isTVar i t
  -> t    = TVar i.
 Proof.
  intros.
  destruct t; snorm; try nope.
+ unfold isTVar in *. snorm.
 Qed.
 Hint Resolve isTVar_form.
 
 
 (* Check whether a type is a region handle with the given index. *)
-Definition isTRgn  (n : nat) (t : ty) : bool
- := match t with
-    | TRgn n' => beq_nat n n'
-    | _       => false
-    end.
+Definition isTRgn_b (n : nat) (t : ty) :=
+ match t with
+ | TRgn n' => beq_nat n n'
+ | _       => false
+ end.
+
+
+Definition isTRgn   (n : nat) (t : ty) 
+ := isTRgn_b n t = true.
+Hint Unfold isTRgn.
 
 
 (* If we know a tpye is a region handle, then it is one.. *)
 Lemma isTRgn_form
  :  forall i t
- ,  true = isTRgn i t
+ ,  isTRgn i t
  -> t    = TRgn i.
 Proof.
  intros.
  destruct t; snorm; try nope.
-  destruct t. snorm. subst. auto.
+ destruct t. unfold isTRgn in *. snorm. subst. auto.
 Qed.
 Hint Resolve isTRgn_form.
 
 
 (* Check whether a type is an effect on the given region variable. *)
-Definition isEffectOnVar (n : nat) (t : ty) : bool
- := match t with
-    | TCon1 tc t1 => andb (isEffectTyCon tc) (isTVar n t1)
-    | _           => false
-    end.
+Definition isEffectOnVar_b (n : nat) (t : ty) := 
+ match t with
+ | TCon1 tc t1 => andb (isEffectTyCon_b tc) (isTVar_b n t1)
+ | _           => false
+ end.
 
 
 (* Check whether a type is an effect on the given region handle. *)
-Definition isEffectOnCap (n : nat) (t : ty) : bool
- := match t with 
-    | TCon1 tc t1 => andb (isEffectTyCon tc) (isTRgn n t1)
-    | _           => false
-    end.
+Definition isEffectOnCap_b (n : nat) (t : ty) :=
+ match t with 
+ | TCon1 tc t1 => andb (isEffectTyCon_b tc) (isTRgn_b n t1)
+ | _           => false
+ end.
 
