done/Iron/Language/SystemF2Effect/Type/Exp/TyCon.v
@@ -11,79 +11,80 @@ Require Export Iron.Language.SystemF2Effect.Kind.
 (********************************************************************)
 (* Type Constructors. *)
 Inductive tycon0 : Type :=
-  | TyConFun    : tycon0
-  | TyConUnit   : tycon0
-  | TyConBool   : tycon0
-  | TyConNat    : tycon0.
+ | TyConFun    : tycon0
+ | TyConUnit   : tycon0
+ | TyConBool   : tycon0
+ | TyConNat    : tycon0.
 Hint Constructors tycon0.
 
 
 Fixpoint kindOfTyCon0 (tc : tycon0) :=
-  match tc with
-  | TyConFun      => KFun KData (KFun KEffect (KFun KData KData))
-  | TyConUnit     => KData
-  | TyConBool     => KData
-  | TyConNat      => KData
-  end.
+ match tc with
+ | TyConFun     => KFun KData (KFun KEffect (KFun KData KData))
+ | TyConUnit    => KData
+ | TyConBool    => KData
+ | TyConNat     => KData
+ end.
 
 
 Fixpoint tycon0_beq tc1 tc2 :=
-  match tc1, tc2 with
-  | TyConFun,       TyConFun    => true
-  | TyConUnit,      TyConUnit   => true
-  | TyConBool,      TyConBool   => true
-  | TyConNat,       TyConNat    => true
-  | _,              _           => false
-  end.
+ match tc1, tc2 with
+ | TyConFun,    TyConFun    => true
+ | TyConUnit,   TyConUnit   => true
+ | TyConBool,   TyConBool   => true
+ | TyConNat,    TyConNat    => true
+ | _,           _           => false
+ end.
 
 
 (********************************************************************)
 (* Type constructors with at least one applied argument. *)
 Inductive tycon1 : Type :=
-  | TyConRead   : tycon1
-  | TyConWrite  : tycon1
-  | TyConAlloc  : tycon1.
+ | TyConRead   : tycon1
+ | TyConWrite  : tycon1
+ | TyConAlloc  : tycon1.
 
 
 Fixpoint kindOfTyCon1 (tc : tycon1) :=
-  match tc with   
-  | TyConRead     => KFun KRegion KEffect
-  | TyConWrite    => KFun KRegion KEffect
-  | TyConAlloc    => KFun KRegion KEffect
-  end.
+ match tc with   
+ | TyConRead    => KFun KRegion KEffect
+ | TyConWrite   => KFun KRegion KEffect
+ | TyConAlloc   => KFun KRegion KEffect
+ end.
 
 
 Fixpoint tycon1_beq tc1 tc2 :=
-  match tc1, tc2 with
-  | TyConRead,   TyConRead   => true
-  | TyConWrite,  TyConWrite  => true
-  | TyConAlloc,  TyConAlloc  => true
-  | _,           _           => false
-  end.
+ match tc1, tc2 with
+ | TyConRead,   TyConRead   => true
+ | TyConWrite,  TyConWrite  => true
+ | TyConAlloc,  TyConAlloc  => true
+ | _,           _           => false
+ end.
 
 
-Definition isEffectTyCon (tc : tycon1) : bool :=
-  match tc with
-  | TyConRead              => true
-  | TyConWrite             => true
-  | TyConAlloc             => true
-  end.
+Definition isEffectTyCon_b (tc : tycon1) :=
+ match tc with
+ | TyConRead     => true
+ | TyConWrite    => true
+ | TyConAlloc    => true
+ end.
 
 
 (********************************************************************)
 (* Type constructors with at least two applied arguments. *)
 Inductive tycon2 : Type :=
-  | TyConRef    : tycon2.
+ | TyConRef    : tycon2.
 Hint Constructors tycon2.
 
 
 Fixpoint kindOfTyCon2 (tc : tycon2) :=
-  match tc with
-  | TyConRef      => KFun KRegion (KFun KData KData)
-  end.
+ match tc with
+ | TyConRef      => KFun KRegion (KFun KData KData)
+ end.
 
 
 Fixpoint tycon2_beq tc1 tc2 :=
-  match tc1, tc2 with
-  | TyConRef,       TyConRef       => true
-  end.
+ match tc1, tc2 with
+ | TyConRef,     TyConRef  => true
+ end.
+
