done/Iron/Language/SystemF2Effect/Type/Relation.v
@@ -6,4 +6,5 @@ Require Export Iron.Language.SystemF2Effect.Type.Relation.EquivTs.
 Require Export Iron.Language.SystemF2Effect.Type.Relation.SubsT.
 Require Export Iron.Language.SystemF2Effect.Type.Relation.SubsTs.
 Require Export Iron.Language.SystemF2Effect.Type.Relation.SubsVisibleT.
+Require Export Iron.Language.SystemF2Effect.Type.Relation.FreeT.
 Require Export Iron.Language.SystemF2Effect.Type.Relation.FreshT.
