done/Iron/Language/SystemF2Effect/Type/Relation/FreeT.v
@@ -1,0 +1,89 @@
+
+Require Export Iron.Language.SystemF2Effect.Type.Exp.
+Require Export Iron.Language.SystemF2Effect.Type.Relation.WfT.
+Require Import Coq.Bool.Bool.
+
+
+(********************************************************************)
+(* Type variable is free in type *)
+Fixpoint freeT (n : nat) (tt: ty)  {struct tt} := 
+ match tt with
+ | TVar ix        => n = ix
+ | TForall k t    => freeT (S n) t
+ | TApp t1 t2     => freeT n t1 \/ freeT n t2
+ | TSum t1 t2     => freeT n t1 \/ freeT n t2
+ | TBot k         => False
+
+ | TCon0 tc       => False
+ | TCon1 tc t1    => freeT n t1
+ | TCon2 tc t1 t2 => freeT n t1 \/ freeT n t2
+ | TCap _         => False
+ end.
+
+
+(********************************************************************)
+Lemma freeT_wfT
+ :  forall n1 n2 t
+ ,  n2 >= n1
+ -> WfT n1 t
+ -> ~freeT n2 t.
+Proof.
+ intros. gen n1 n2.
+ induction t; intros; inverts H0;
+  unfold not; intros; snorm; subst; try omega.
+
+ - cut (~ freeT (S n2) t); firstorder.
+
+ - inverts H0.
+   cut (~ freeT n2 t1); firstorder.
+   cut (~ freeT n2 t2); firstorder.
+ 
+ - inverts H0.
+   cut (~ freeT n2 t1); firstorder.
+   cut (~ freeT n2 t2); firstorder.
+
+ - cut (~ freeT n2 t0); firstorder.
+
+ - inverts H0.
+   cut (~ freeT n2 t2); firstorder.
+   cut (~ freeT n2 t3); firstorder.
+Qed.
+Hint Resolve freeT_wfT.
+
+
+Lemma freeT_closedT
+ :  forall t n
+ ,  ClosedT t
+ -> ~freeT n t.
+Proof.
+ intros. 
+ eapply freeT_wfT; eauto.
+Qed.
+
+
+Lemma freeT_wfT_drop
+ :  forall n t
+ ,  WfT (S n) t
+ -> ~freeT n t
+ -> WfT  n    t.
+Proof.
+ intros. gen n.
+ induction t; snorm; inverts H; firstorder.
+Qed.
+
+
+Lemma freeT_isEffectOnVar
+ :  forall d t
+ ,  ~(freeT d t)
+ -> isEffectOnVar_b d t = false.
+Proof.
+ intros. 
+ destruct t; snorm.
+ destruct t0; snorm;
+  try (solve [rewrite andb_false_iff; tauto]).
+
+ - rewrite andb_false_iff. right. 
+   rewrite beq_nat_false_iff. auto.
+Qed.
+Hint Resolve freeT_isEffectOnVar.
+
